RelConfig.v
@@ -173,27 +173,33 @@ Definition S_builtin_ins :=
       sfree 4; ret];
    raise_loc !->c
      ins_seq
-     [load r4 r1 0; store r1 0 sp;
-      mov sp r4; load r5 r1 3;
-      malloc r3 1; store r3 0 r1;
-      load r1 r1 2; call r5;
+     [load r4 r1 false 1; (*r4 <- L_prev^|s_prev|*)
+      store r1 false 1 sp; (*L_prev^|s_prev| -> cursp*)
+      mov sp r4; (*sp <- L_prev^|s_prev|*)
+      load r5 r1 false 4;(*r5 <- P_op*)
+      malloc r3 1;store r3 true 0 r1;(*make heap tuple for L_rsp*)
+      load r1 r1 false 3;(*r1 <- L_env*)
+      call r5;
       ret];
    resume_loc !->c
      ins_seq
-     [load r3 r1 0; store r1 0 ns;
-      load r4 r3 0; store r3 0 sp;
-      mov r1 r2; mov sp r4;
-      ret];
+     [(*rewrite the tuple for L_rsp*)
+       load r3 r1 true 0; store r1 true 0 ns;
+       (*replace L^|s| in continuation*)
+       load r4 r3 false 1;store r3 false 1 sp;
+       mov r1 r2; mov sp r4;
+       ret];
    c_empty).
 
 Definition ns_hdl_lab : L.hdl_label := hdl_lab ""%string.
+Definition ns_obj_lab : L.obj_label := obj_lab ""%string.
 Definition ns_clab : L.code_label := ""%string.
 Inductive init_L :
   L.code_mem -> (L.code_mem * L.heap * L.eval_context
                 * L.local_env * L.term) -> Prop :=
 | mk_init_L : forall (C:L.code_mem) (H:L.heap) dummy_hdl,
     dummy_hdl = h_f (handler_f ns_hdl_lab
-                       ns_hdl_lab ns_clab general) ->
+                       ns_obj_lab ns_clab general) ->
     (forall (x:string) n t,
         L.c_comp L_init_func C x = func n t ->
         S_builtin_ins x = ns_ins_seq) ->
@@ -201,13 +207,16 @@ Inductive init_L :
     init_L C
       (L.c_comp L_init_func C,
         L.h_empty, [dummy_hdl] ,[], L_init_tm)%L_scope.
-Definition ns_hloc : S.word := hloc ""%string 0.
+Definition ns_hloc_str : S.heap_loc := hloc_str ""%string.
+Definition ns_hloc : S.word := hloc ns_hloc_str 0.
+Definition ns_hdl_hloc : S.word := hloc ns_hloc_str 4.
 Definition ns_cloc : S.word := cloc ""%string 0.
 Inductive init_S : S.code_mem ->
   (S.code_mem * S.heap * reg_file) -> Prop :=
-| mk_init_S : forall (uc:code_mem) L_stack dummy_hdl_stk,
+| mk_init_S : forall (uc:code_mem) dummy_hdl_stk,
     (* a stack section as a dummy handler *)
-    dummy_hdl_stk = [ns_hloc;int_w 0;ns_hloc;ns_cloc] ->
+    dummy_hdl_stk = [loc_w (cloc handle_loc 10);
+                     ns_hdl_hloc;int_w 0;ns_hloc;ns_cloc] ->
     (forall LC x,
         uc = code_mem_trans LC ->
         wf_func_tm (LC x)) ->
@@ -216,8 +225,8 @@ Inductive init_S : S.code_mem ->
         S_builtin_ins x = ns_ins_seq) ->
     init_S
       uc (c_comp S_builtin_ins (c_comp S_init_ins uc),
-        ([(L_stack,stack dummy_hdl_stk)],th_empty,(sh_empty, th_empty)),
-        [(ip,loc_w (cloc init_lab 0));(sp,loc_w (hloc L_stack 4));
+        ([(ns_hloc_str,stack dummy_hdl_stk)] ++ [],th_comp th_empty th_empty),
+        [(ip,loc_w (cloc init_lab 0));(sp,loc_w (hloc ns_hloc_str 5));
          (r0,ns);(r1,ns);
          (r2,ns);(r3,ns);(r4,ns);
          (r5,ns);(r6,ns)]).
@@ -228,11 +237,15 @@ Inductive final_L : (L.code_mem * L.heap * L.eval_context *
   mk_final_L : forall C H K (i:nat),
     final_L (C,H,K,[run_const i],L.halt) i.
 Inductive final_S : (S.code_mem * S.heap * reg_file) -> word -> Prop :=
-  mk_final_S : forall p H_stk H_conts H_tup R (l:code_location)
-    (i:nat) lsp S,
+| mk_final_S :
+  forall p H_stk H_tup H_cont H_ctup R (l:code_location)
+         (i:nat) lsp S,
     fetch_instr l p = halt ->
-    final_S (p,((lsp,stack ((int_w i) :: S)):: H_stk,H_tup,H_conts),
-    [(ip,loc_w l);(sp,loc_w (hloc lsp (1 + (List.length S))))] ++ R) i.
+    final_S (p,((lsp,stack ((int_w i) :: S)) :: H_stk ++ H_cont,
+                 th_comp H_tup H_ctup),
+        [(ip,loc_w l);
+         (sp,loc_w (hloc lsp (1 + (List.length S))))]
+          ++ R) i.
 
 
 (* ----------------------------------------------------------
@@ -242,20 +255,42 @@ Inductive LS_rel_run_cst :
   L.runtime_const -> S.word -> Prop :=
 | rel_run_cst :
   forall cst, LS_rel_run_cst cst (run_cst_trans cst).
-                     
-Inductive LS_rel_run_csts :
+Definition run_cstlst_trans
+  (lstv:list L.runtime_const) : list S.word :=
+  List.map run_cst_trans lstv.
+Inductive LS_rel_run_cstlst :
   list L.runtime_const -> list S.word -> Prop :=
 | rel_run_csts : forall lstv,
-    LS_rel_run_csts lstv (List.map run_cst_trans lstv).
-
+    LS_rel_run_cstlst lstv (run_cstlst_trans lstv).
+Definition env_trans
+  (lstv:L.local_env) : S.stack_heap_val :=
+  stack (run_cstlst_trans lstv).
 Inductive LS_rel_env : L.local_env -> S.stack_heap_val -> Prop :=
 | rel_env : forall envlst,
-    LS_rel_env envlst (stack (List.map run_cst_trans envlst)).
+    LS_rel_env envlst (env_trans envlst).
+Definition ins_trans (E:L.local_env) (t:L.term) :
+  S.instr_seq :=
+  ins_seq (LS.func_term_trans (List.length E) t).
 Inductive LS_rel_ins : (L.local_env*L.term) -> S.instr_seq -> Prop :=
 | rel_ins : forall E t,
     wf_tm E t ->
     LS_rel_ins (E,t)
-      (ins_seq (LS.func_term_trans (List.length E) t)).
+      (ins_trans E t).
+(*Definition frame_trans (af:L.a_frame) : S.stack_heap_val :=
+  match af with
+  | act_f E t =>
+      stack ((loc_w (cloc C_lab (List.length lst)))
+               :: (run_cst_trans E))
+  end.
+Inductive LS_rel_frame (C_mem : S.code_mem): L.a_frame -> S.stack_heap_val -> Prop :=
+| rel_frame : forall E t Ilst C_lab i lst s,
+    LS_rel_ins (L.ns :: E,t) (ins_seq (tl Ilst))
+    -> C_mem C_lab = ins_seq (lst ++ Ilst)
+    -> nth 0 Ilst halt = push r1 ->
+    
+    LS_rel_frame C_mem (act_f E t)
+      (stack ((loc_w (cloc C_lab i)) :: s)).*)
+
 Inductive LS_rel_frame (C_mem : S.code_mem): L.a_frame -> S.stack_heap_val -> Prop :=
   rel_frame : forall E t Ilst C_lab i lst s,
     LS_rel_ins (L.ns :: E,t) (ins_seq (tl Ilst))
@@ -271,64 +306,69 @@ Inductive LS_rel_frames (C_mem : S.code_mem) : (list L.frame)
     LS_rel_frame C_mem Fi (stack si)
     -> LS_rel_frames C_mem Flst (stack s')
     -> LS_rel_frames C_mem ((a_f Fi) :: Flst) (stack (si ++ s')).
-Inductive LS_rel_hdl : L.h_frame -> list S.word -> Prop :=
-| rel_hdl_general : forall (L L_env Clab_op:string) L_prev (s_prev:list word),
-    LS_rel_hdl
+Inductive LS_rel_hdl (L : string)
+  : L.h_frame -> list S.word -> Prop :=
+| rel_hdl_general : forall (L_env Clab_op:string) L_prev (s_prev:list word),
+    LS_rel_hdl L
       (handler_f (hdl_lab L)
-              (hdl_lab L_env) Clab_op general)
-      [loc_w (hloc L_prev (List.length s_prev));
+              (obj_lab L_env) Clab_op general)
+      [loc_w (cloc handle_loc 10);
+       loc_w (hloc L_prev (List.length s_prev));
        int_w 0; loc_w (hloc L_env 0);
        loc_w (c_loc (cloc Clab_op 0))]
-| rel_hdl_other : forall (L L_env Clab_op:string) A num,
+| rel_hdl_other : forall (L_other L_env Clab_op:string) A num,
     (A = tail -> num = 1) -> (A = abort -> num = 2) ->
-    LS_rel_hdl
-      (handler_f (hdl_lab L)
-              (hdl_lab L_env) Clab_op A)
-      [ns; int_w num; loc_w (hloc L_env 0);
+    A = tail \/ A = abort ->
+    LS_rel_hdl L
+      (handler_f (hdl_lab L_other)
+              (obj_lab L_env) Clab_op A)
+      [loc_w (cloc handle_sm_stk_loc 8);
+       ns; int_w num; loc_w (hloc L_env 0);
        loc_w (c_loc (cloc Clab_op 0))].
-Definition is_general_hdl_frame (f:L.h_frame) : bool :=
+Definition is_h_frm_general_hdl (f:L.h_frame) : bool :=
   match f with
   | handler_f _ _ _ general => true
   | _ => false
   end.
-Inductive LS_rel_hdl_stk (C_mem : S.code_mem) :
+Definition is_frm_general_hdl (f:L.frame):bool :=
+  match f with
+  | handler_f _ _ _ general => true
+  | _ => false
+  end.
+Inductive LS_rel_hdl_stk
+  (C_mem : S.code_mem) (L : string) :
   list L.frame -> list S.word -> Prop :=
 | rel_hdl_stk_base : forall Flst s frm frm_stk,
     LS_rel_frames C_mem Flst (stack s) ->
-    LS_rel_hdl frm frm_stk ->
-    is_general_hdl_frame frm = true ->
-    LS_rel_hdl_stk C_mem (Flst ++ [h_f frm]) (s ++ frm_stk)
+    LS_rel_hdl L frm frm_stk ->
+    is_h_frm_general_hdl frm = true ->
+    LS_rel_hdl_stk C_mem L (Flst ++ [h_f frm]) (s ++ frm_stk)
 | rel_hdl_stk : forall Flst s frm frm_stk Klst slst,
-    LS_rel_hdl_stk C_mem Klst slst ->
+    LS_rel_hdl_stk C_mem L Klst slst ->
     LS_rel_frames C_mem Flst (stack s) ->
-    LS_rel_hdl frm frm_stk ->
-    is_general_hdl_frame frm = false ->
-    LS_rel_hdl_stk C_mem (Flst ++ [h_f frm] ++ Klst) (s ++ frm_stk ++ slst).
+    LS_rel_hdl L frm frm_stk ->
+    is_h_frm_general_hdl frm = false ->
+    Klst <> [] /\ slst <> [] ->
+    LS_rel_hdl_stk C_mem L (Flst ++ [h_f frm] ++ Klst) (s ++ frm_stk ++ slst).
 (* ensures that each stack in the list of stacks
    relates to the corresponding frames of K, in
    the same and correct order
    
    also ensures that all stacks except the first one
    should point to the previous stack*)
-Inductive LS_rel_hdl_stk_lst (C_mem : S.code_mem):
-  list L.frame -> list (S.heap_loc * S.stack_heap_val) -> Prop :=
-| rel_hdl_stk_nil : LS_rel_hdl_stk_lst C_mem [] []
-| rel_hdl_stk_lst : forall Ks H K s L,
-    LS_rel_hdl_stk_lst C_mem Ks H ->
-    LS_rel_hdl_stk C_mem K s ->
-    LS_rel_hdl_stk_lst C_mem (K ++ Ks) ((L,stack s)::H).
 Definition stk_points_to
-  (s s_prev:list S.word) (L:string) :=
+  (s s_prev:list S.word) (L:heap_loc) :=
   nth_error (rev s) 3 = Some (loc_w (hloc L (List.length s_prev))).
-(* must have at least 1 stack *)
 Inductive LS_rel_eval_ctx (C_mem : S.code_mem) :
   L.eval_context -> S.stack_heap -> Prop :=
-| rel_hdl_led_ctx : forall Ks H,
-    (forall L s s' L' H',
-        H = [(L,stack s);(hloc_str L',stack s')] ++ H' ->
+| rel_eval_ctx_nil : LS_rel_eval_ctx C_mem [] []
+| rel_eval_ctx_lst : forall Ks H K s L,
+    LS_rel_eval_ctx C_mem Ks H ->
+    LS_rel_hdl_stk C_mem L K s ->
+    (forall L' s' H',
+        H = (L',stack s') :: H' -> 
         stk_points_to s s' L') ->
-    LS_rel_hdl_stk_lst C_mem Ks H ->
-    LS_rel_eval_ctx C_mem Ks H.
+    LS_rel_eval_ctx C_mem (K ++ Ks) ((hloc_str L,stack s)::H).
 
 Inductive LS_rel_env_context (C_mem : S.code_mem) : (L.eval_context * L.local_env) ->
   (S.stack_heap * S.heap_location) -> Prop :=
@@ -346,50 +386,43 @@ Inductive LS_rel_tup_heap : L.tup_heap -> S.tuple_heap -> Prop :=
         LH_tup (obj_lab L_tup) = L.tuple vs
         -> SH_tup L_tup = tuple (List.map run_cst_trans vs)) ->
     LS_rel_tup_heap LH_tup SH_tup.
-(*
-  
-Inductive LS_rel_cont_stks :
-  list L.frame -> S.stack_heap -> Prop :=
-  rel_cont_stks :
-    LS_rel_hdl_led_ctx Ks H_one_cont ->
-    H_one_cont =
-      [(L_last, stack (s_last))]
-        ++ stks ++
-        [stack (s_0 ++ [loc_w (hloc L_last (List.length s_last));
-                          int_w 0; loc_w (hloc L_env 0);
-                          loc_w (c_loc (cloc Clab_op 0))])]
-                                                          
-Inductive LS_rel_cont_heap :
+Inductive LS_rel_cont (C_mem : S.code_mem) :
+  L.heap_cont -> S.stack_heap -> Prop :=
+| rel_cont_stks :
+  forall Ks H L_fst s_fst L_lst s_lst stks,
+  LS_rel_eval_ctx C_mem Ks H ->
+  H = (L_fst, stack s_fst)
+        :: stks ++ [(L_lst, stack s_lst)] ->
+  stk_points_to s_lst s_fst L_fst ->
+  LS_rel_cont C_mem (cont Ks) H.
+Inductive LS_rel_cont_heap (C_mem : S.code_mem) :
   L.cont_heap -> (S.stack_heap * S.tuple_heap) -> Prop :=
-  rel_cont_heap :
-    forall LH_cont SH_cont (SH_ctup:S.tuple_heap),
-      (forall (L_rsp:string) (L:string) L_out L_env  
-              s s_out Ks Clab_op,
-          LH_cont (obj_lab L_rsp) = cont Ks ->
-          Ks = ([h_f (handler_f (hdl_lab L_out) (hdl_lab L_env')
-                        (c_lab Clab_op') general)]
-                  ++ Ks_middle ++
-                  [h_f (handler_f (hdl_lab L) (hdl_lab L_env)
-                          (c_lab Clab_op) general)]) ->
-          LS_rel_hdl_led_ctx Ks SH_cont ->
-          SH_ctup L_rsp = tuple [loc_w (hloc L 4)]
-          /\ stk_heap_app SH_cont L_out = stack s_out
-          /\ stk_heap_app SH_cont L =
-           stack (s ++ [loc_w (hloc L_out (List.length s_out));
-                        int_w 0;loc_w (hloc L_env 0);loc_w (cloc Clab_op 0)]))
-      -> LS_rel_cont_heap LH_cont (SH_cont,SH_ctup).*)
+| rel_cont_heap :
+  forall LH_cont SH_cont (SH_ctup:S.tuple_heap),
+    (forall (L_rsp:string) L_last
+            H_one_cont H_one_cont_ld
+            H_conts_ld  H_conts_ed s_last,
+        LS_rel_cont C_mem (LH_cont (obj_lab L_rsp)) H_one_cont ->
+        H_one_cont = H_one_cont_ld ++ [(L_last,stack s_last)] ->
+        SH_cont = H_conts_ld ++ H_one_cont ++ H_conts_ed
+        /\ SH_ctup L_rsp = tuple [loc_w (hloc L_last 4)]) ->
+    LS_rel_cont_heap C_mem LH_cont (SH_cont,SH_ctup).
 (* each continuation is a list of stacks, like H_stk.
    The difference is that the first stack doesn't point
    back to the context frame where it was cut off, but rather
    circularly points to the last stack of this continuation.*)
-Inductive LS_rel_heap :
+Inductive LS_rel_heap (C_mem : S.code_mem) :
   L.heap -> (S.stack_heap * tuple_heap * tuple_heap) -> Prop :=
   rel_heap :
   forall LH_tup SH_tup
-         (SH_conts:stack_heap * tuple_heap) (LH_cont:L.cont_heap),
+         (SH_conts:stack_heap * tuple_heap)
+         (LH_cont:L.cont_heap),
     LS_rel_tup_heap LH_tup SH_tup ->
-    (* LS_rel_cont_heap LH_cont SH_conts -> *)
-    LS_rel_heap (LH_tup,LH_cont) (SH_conts,SH_tup).
+    LS_rel_cont_heap C_mem LH_cont SH_conts ->
+    (forall (x:string) e lst,
+        LH_tup (obj_lab x) = L.tuple (e :: lst) ->
+        SH_tup x <> tuple []) ->
+    LS_rel_heap C_mem (LH_tup,LH_cont) (SH_conts,SH_tup).
 Inductive LS_rel_code_mem : L.code_mem -> S.code_mem -> Prop :=
 | rel_code : forall LC SC,
     SC = code_mem_trans LC ->
@@ -398,9 +431,6 @@ Inductive LS_rel_code_mem : L.code_mem -> S.code_mem -> Prop :=
         LC x = func n t ->
         S_builtin_ins x = ns_ins_seq) ->
     LS_rel_code_mem LC SC.
-(* | rel_code_func : forall f (x:string) C,
-    LS_rel_code (x !->c f ; C)%L_scope
-      (cloc_str x !->c func_trans f; (code_trans C)).*)
 (* A runtime lexi config relates to a runtime salt config if
    subparts of the configs relates to each other accordingly,
    and that the lexi term t is locally closed (i.e. without
@@ -417,19 +447,20 @@ Inductive LS_rel :
   -> (S.code_mem * S.heap * reg_file) -> Prop :=
   rel_LS : forall len lst SIlst
     LC LH LK LE Lt SC o0 o1 o2 o3 o4 o5 o6
-    (SH_stack:stack_heap) (SH_conts:stack_heap * tuple_heap)
-    (SH_tup:tuple_heap)
+    (SH_stack SH_cont:stack_heap)
+    (SH_tup SH_ctup:tuple_heap)
     (Slsp:heap_location) Clab,
     LS_rel_ins (LE,Lt) (ins_seq SIlst) ->
     LS_rel_env_context (c_comp S_builtin_ins SC)
       (LK,LE) (SH_stack,Slsp) ->
-    LS_rel_heap LH (SH_conts,SH_tup) ->
+    LS_rel_heap SC LH ((SH_cont,SH_ctup),SH_tup) ->
     LS_rel_code_mem LC SC ->
     (c_comp S_builtin_ins SC) Clab = ins_seq (lst ++ SIlst) ->
     List.length lst = len ->
     (*lc_term Lt \/ body Lt*)
     LS_rel (LC, LH, LK, LE, Lt)
-      (c_comp S_builtin_ins SC, (SH_stack,SH_tup,SH_conts),
+      (c_comp S_builtin_ins SC,
+        (SH_stack ++ SH_cont,th_comp SH_tup SH_ctup),
         [(ip,loc_w (cloc Clab len));(sp,loc_w Slsp);
          (r0,o0);(r1,o1);
          (r2,o2);(r3,o3);(r4,o4);
@@ -442,4 +473,9 @@ the rules for hdl-led ctx needs to be changed
 handlers are on top not bottom, syntax wrong
   other than this the whole rules need to change
 
+
+built in raise instruction sequence have 1 offset
+wrong, and they should all be load _ [_-_], not
+load _ [_+_] (same for store), because you go 
+down the stack
 *)
